Write theorems and proofs for loop-free programs.

src/LoopFormalization/LRelationalAbstractInterpreter.v
@@ -34,19 +34,19 @@ Section AbstractInterpreter.
     else
       true.
 
-  Fixpoint abstract_interpret_inst_list (state: AbstractState) (l: list Inst) (bb_id: bbid) (pos: nat) :=
+  Fixpoint abstract_interpret_inst_list (l: list Inst) (bb_id: bbid) (pos: nat) (state: AbstractState) :=
     match l with
     | nil => state
     | inst::l' => let new_ab := transfer_inst inst (state bb_id pos) in
                 let new_state := (bb_id !-> (S pos !-> new_ab; state bb_id); state) in
-                abstract_interpret_inst_list new_state l' bb_id (S pos)
+                abstract_interpret_inst_list l' bb_id (S pos) new_state
     end.
 
   Theorem abstract_interpret_inst_list_spec (bb: BasicBlock) (bb_id: bbid):
     Some bb = p bb_id ->
     forall (l: list Inst) pos, (forall n, nth_error l n = nth_error bb.1.2 (n + pos)) ->
       forall state, (forall n', n' < pos -> inst_fixpoint state bb_id n') ->
-        forall n'', inst_fixpoint (abstract_interpret_inst_list state l bb_id pos) bb_id n''.
+        forall n'', inst_fixpoint (abstract_interpret_inst_list l bb_id pos state) bb_id n''.
   Proof.
     move => Hbb.
     elim => [ /= pos Hnth state Hfixpoint n''| inst l Hind pos Hnth state Hfixpoint n'' /=].
@@ -78,5 +78,261 @@ Section AbstractInterpreter.
         apply /eqP.
         auto.
   Qed.
+
+  Theorem abstract_interpret_inst_list_0_unchanged (l: list Inst) (bb_id bb_id': bbid) (pos: nat) (state: AbstractState) :
+  state bb_id' 0 = (abstract_interpret_inst_list l bb_id pos state) bb_id' 0.
+  Proof.
+    elim: l state pos => [ // | i l Hind state pos].
+    case (bb_id' =P bb_id) => [Heq | /eqP Hne].
+    - rewrite Heq in Hind *.
+      rewrite -Hind.
+        by simpl_totalmap.
+    - rewrite -Hind.
+        by simpl_totalmap.
+  Qed.
+
+  Theorem abstract_interpret_inst_list_bb_unchanged (l: list Inst) (bb_id: bbid) :
+    forall bb_id', bb_id != bb_id' ->
+              forall state pos n, (abstract_interpret_inst_list l bb_id pos state) bb_id' n = state bb_id' n.
+  Proof.
+    move => bb_id' Hbb_ne.
+    elim: l => [ // | i l Hind state pos n /=].
+    rewrite Hind.
+      by simpl_totalmap.
+  Qed.
+
+  Definition abstract_interpret_join_term_succ (state: AbstractState) (abs: list (ab * bbid)) :=
+    fold_right (fun abid state =>
+               match abid with
+               | (ab, out_id) => (out_id !-> (O !-> join ab (state out_id O); state out_id); state)
+               end
+               ) state abs.
+
+  Lemma abstract_interpret_join_term_unchanged (state: AbstractState) (abs: list (ab * bbid)) (bb_id: bbid) (pos: nat) :
+    pos != O -> (abstract_interpret_join_term_succ state abs) bb_id pos = state bb_id pos.
+  Proof.
+    move => Hpos.
+    elim: abs => [ // | [a out_id] l Hind ].
+    case (out_id =P bb_id) => [-> | Hne]; by simpl_totalmap.
+  Qed.
+
+  Lemma abstract_interpret_join_term_bb_unchanged (bb_id: bbid):
+    forall abs, (forall a', not (In (a', bb_id) abs)) ->
+           forall state pos, (abstract_interpret_join_term_succ state abs) bb_id pos = state bb_id pos.
+  Proof.
+    move => HnotIn.
+    elim: HnotIn => [// | [a out_id] abs' Hind /=].
+    case (bb_id =P out_id) => [<- /(_ a) /Decidable.not_or [Himpossible _]// | Hne HnotIn].
+    have: (forall a', ~ In (a', bb_id) abs'). by move => a'; move: HnotIn => /(_ a') /Decidable.not_or[_ Hgoal].
+    move => HnotIn' state pos.
+    apply Hind with (state := state) (pos := pos) in HnotIn'.
+      by simpl_totalmap.
+  Qed.
+
+  Lemma abstract_interpret_join_term_monotone (state: AbstractState) (abs: list (ab * bbid)) (bb_id: bbid) (pos: nat) :
+    le (state bb_id pos) ((abstract_interpret_join_term_succ state abs) bb_id pos).
+  Proof.
+    elim: abs => [ /= | [a' bb] l /=]. by apply AbstractDomain.le_refl.
+    case (bb_id =P bb) => [-> | Hne Hind]; [ | by simpl_totalmap].
+    case pos => [Hind | n Hind]; [ |by simpl_totalmap].
+    simpl_totalmap.
+    eapply AbstractDomain.le_trans; eauto.
+    apply join_sound_r.
+  Qed.
+
+  Lemma abstract_interpret_join_term_join (abs: list (ab * bbid)) (a: ab) (bb_id: bbid) :
+    In (a, bb_id) abs ->
+    forall state, le a ((abstract_interpret_join_term_succ state abs) bb_id O).
+  Proof.
+    elim: abs => [// | [a0 out_id] l Hind /= [[-> ->] | HIn] state].
+    - simpl_totalmap. apply join_sound_l.
+    - case (out_id =P bb_id) => [-> | Hne].
+      + simpl_totalmap.
+        eapply AbstractDomain.le_trans.
+        * by apply Hind.
+        * apply join_sound_r.
+      + simpl_totalmap. auto.
+  Qed.
+
+  Definition abstract_interpret_term (bb: BasicBlock) (bb_id: bbid) (state: AbstractState) :=
+    let pos := length bb.1.2 in
+    let new_abs := transfer_term bb.2 (state bb_id pos) in
+    abstract_interpret_join_term_succ state new_abs.
+
+  Theorem abstract_interpret_term_spec (bb: BasicBlock) (bb_id: bbid) (state: AbstractState):
+    Some bb = p bb_id ->
+    ~~(list_string_in (term_successors bb.2) bb_id) ->
+    term_fixpoint (abstract_interpret_term bb bb_id state) bb_id.
+  Proof.
+    move => Hbb Hbbnotsucc. rewrite /term_fixpoint -Hbb.
+    apply forallb_forall => [[a out_id]].
+    rewrite /abstract_interpret_term.
+    move: Hbbnotsucc.
+    move Hterm: bb.2 => term Hbbnotsucc.
+    move Hpos: (length bb.1.2) => pos.
+    move Htransfer: (transfer_term term ((state bb_id) pos)) => transfer.
+    case (pos =P 0) => [Heq | /eqP Hne]; last first.
+    - rewrite abstract_interpret_join_term_unchanged => [ | //].
+      rewrite Htransfer => HIn.
+        by apply abstract_interpret_join_term_join.
+    - rewrite Heq in Hpos Htransfer *.
+      case (out_id =P bb_id) => [-> HIn | Hne].
+      + have: (list_string_in (term_successors term) bb_id) => [ | Hcontra].
+        * eapply transfer_term_only_successors.
+          eauto.
+        * by rewrite Hcontra in Hbbnotsucc.
+      + move: (abstract_interpret_join_term_bb_unchanged bb_id transfer).
+        have: (forall a' : ab, ~ In (a', bb_id) transfer).
+        * move => a' HIn.
+          rewrite -Htransfer in HIn.
+          move: (@transfer_term_only_successors ab ad tf term bb_id (state bb_id 0)).
+          have: ((exists a'0 : ab, In (a'0, bb_id) (transfer_term term ((state bb_id) 0)))). by (exists a').
+          move => HexistsIn /(_ HexistsIn).
+          move => HbbInsucc.
+            by rewrite HbbInsucc in Hbbnotsucc.
+        * move => HnotIn /(_ HnotIn) Hunchanged.
+          rewrite Hunchanged Htransfer => HIn.
+            by apply abstract_interpret_join_term_join.
+  Qed.
+
+  Lemma abstract_interpret_term_monotone (state: AbstractState) (bb: BasicBlock) (bb_id bb_id': bbid) (pos: nat) :
+    le (state bb_id' pos) ((abstract_interpret_term bb bb_id state) bb_id' pos).
+  Proof.
+    rewrite /abstract_interpret_term.
+      by apply abstract_interpret_join_term_monotone.
+  Qed.
+
+  Lemma abstract_interpret_term_bb_unchanged (bb_id: bbid) (bb: BasicBlock):
+    (Some bb = p bb_id) ->
+    forall bb_id', bb_id' != bb_id ->
+              ~~(list_string_in (term_successors bb.2) bb_id') ->
+              forall state pos, (abstract_interpret_term bb bb_id state) bb_id' pos = state bb_id' pos.
+  Proof.
+    move => Hbb bb_id' Hbb_ne Hbb_not_term state pos.
+    rewrite /abstract_interpret_term.
+    rewrite abstract_interpret_join_term_bb_unchanged => [// | a' HIn].
+    have: (list_string_in (term_successors bb.2) bb_id').
+    - eapply transfer_term_only_successors.
+      eauto.
+    - move => Himpossible.
+        by rewrite Himpossible in Hbb_not_term.
+  Qed.
+
+  Definition abstract_interpret_bb (bb: BasicBlock) (bb_id: bbid) (state: AbstractState) :=
+    let state' := abstract_interpret_inst_list bb.1.2 bb_id 0 state in
+    abstract_interpret_term bb bb_id state'.
+
+  Theorem abstract_interpret_bb_spec_term (bb: BasicBlock) (bb_id: bbid) (state: AbstractState) :
+    Some bb = p bb_id ->
+    ~~(list_string_in (term_successors bb.2) bb_id) ->
+    term_fixpoint (abstract_interpret_bb bb bb_id state) bb_id.
+  Proof.
+    move => Hbb HnotIn.
+      by apply abstract_interpret_term_spec.
+  Qed.
+
+  Theorem abstract_interpret_bb_spec_inst (bb: BasicBlock) (bb_id: bbid) (state: AbstractState) :
+    Some bb = p bb_id ->
+    ~~(list_string_in (term_successors bb.2) bb_id) ->
+    (forall n, inst_fixpoint (abstract_interpret_bb bb bb_id state) bb_id n).
+  Proof.
+    move => Hbb HnotIn n.
+    rewrite /abstract_interpret_bb.
+    have: (inst_fixpoint (abstract_interpret_inst_list bb.1.2 bb_id 0 state) bb_id n).
+    - eapply abstract_interpret_inst_list_spec => [| n0 |]; eauto.
+      by rewrite addn0.
+    - case: n => [ H | n H]; last first.
+      + rewrite /inst_fixpoint !abstract_interpret_join_term_unchanged => //.
+      + rewrite /inst_fixpoint (abstract_interpret_join_term_unchanged _ _ _ 1) /abstract_interpret_term => //.
+        rewrite (abstract_interpret_join_term_bb_unchanged bb_id) => //.
+        move => a' HIna'.
+        have: (exists a'0 : ab, In (a'0, bb_id) (transfer_term bb.2 (((abstract_interpret_inst_list bb.1.2 bb_id 0 state) bb_id) (Datatypes.length bb.1.2)))). by eauto.
+        move => HexistsIn.
+        apply transfer_term_only_successors in HexistsIn.
+          by rewrite HexistsIn in HnotIn.
+  Qed.
+
+  Theorem abstract_interpret_bb_monotone_0 (bb: BasicBlock) (bb_id bb_id': bbid) (state: AbstractState):
+    le (state bb_id' 0) ((abstract_interpret_bb bb bb_id state) bb_id' 0).
+  Proof.
+    rewrite /abstract_interpret_bb.
+    erewrite abstract_interpret_inst_list_0_unchanged.
+    apply abstract_interpret_term_monotone.
+  Qed.
+
+  Fixpoint abstract_interpret_program (ps: ProgramStructure) (state: AbstractState) :=
+    match ps with
+    | BB bb_id =>
+      match p bb_id with
+      | Some bb => abstract_interpret_bb bb bb_id state
+      | None => state
+      end
+    | DAG ps1 ps2 =>
+      let state' := abstract_interpret_program ps1 state in
+      abstract_interpret_program ps2 state'
+    | _ => state
+    end.
+
+  Theorem abstract_interpret_program_monotone_0 (ps: ProgramStructure) (state: AbstractState) (bb_id: bbid) :
+    le (state bb_id 0) ((abstract_interpret_program ps state) bb_id 0).
+  Proof.
+    elim: ps state.
+    - admit.
+    - move => ps1 Hind1 ps2 Hind2 state /=.
+      eapply AbstractDomain.le_trans; eauto.
+    - rewrite /abstract_interpret_program => bb state.
+      case: (p bb) => [a | ].
+      + by apply abstract_interpret_bb_monotone_0.
+      + by apply AbstractDomain.le_refl.
+  Admitted.
+
+  Theorem abstract_interpret_program_unchanged (ps: ProgramStructure) :
+    structure_sound p ps ->
+    forall bb_id, ~~(list_string_in (program_successors p ps) bb_id) ->
+             ~~(list_string_in (bbs_in_program ps) bb_id) ->
+             forall state pos, (abstract_interpret_program ps state) bb_id pos = state bb_id pos.
+  Proof.
+    elim: ps.
+    - admit.
+    - move => ps1 Hind1 ps2 Hind2 /= /andP[/andP[_ Hsound1] Hsound2] bb_id.
+      rewrite !list_string_in_append => /norP[Hinsucc1 Hinsucc2] /norP[Hinprog1 Hinprog2] state pos.
+      rewrite Hind2 => //.
+        by rewrite Hind1 => //.
+    - move => bb_id Hsound bb_id' Hnot_in_succ /norP [Hnebb _] state pos /=.
+      case_eq (p bb_id) => [[[params insts] term] | //] => Hbb.
+      rewrite /abstract_interpret_bb.
+      erewrite abstract_interpret_term_bb_unchanged; eauto.
+      rewrite abstract_interpret_inst_list_bb_unchanged => //. by rewrite eq_sym.
+      by rewrite /= Hbb in Hnot_in_succ.
+  Admitted.
+
+  Theorem abstract_interpret_program_spec_term (ps: ProgramStructure):
+    structure_sound p ps ->
+    forall bb_id, list_string_in (bbs_in_program ps) bb_id ->
+             forall state, term_fixpoint (abstract_interpret_program ps state) bb_id.
+  Proof.
+    elim ps => [ | | bb_id' /=].
+    - admit.
+    - move => ps1 Hind1 ps2 Hind2 /= /andP[/andP[/andP[/andP[/andP[H2notin1 H1notin2] Hloops] Hdominance] Hsound1] Hsound2] bb_id.
+      rewrite list_string_in_append => /orP [ HIn1 | HIn2 ] state; auto.
+      have: (term_fixpoint (abstract_interpret_program ps1 state) bb_id) by auto.
+      move => Hfixpoint1.
+      rewrite /term_fixpoint in Hfixpoint1 *.
+      case: (p bb_id) Hfixpoint1 => [ bb Hfixpoint1 | //].
+      apply forallb_forall => [[a bb_id']] HIn.
+      rewrite abstract_interpret_program_unchanged in HIn => //.
+      + eapply forallb_forall with (x := (a, bb_id')) in Hfixpoint1; auto.
+        eapply AbstractDomain.le_trans; eauto.
+        by apply abstract_interpret_program_monotone_0.
+      + move => /list_string_in_spec in HIn1.
+        apply /list_string_in_spec => Hinsucc2.
+        eapply forallb_forall in Hdominance; eauto.
+        move => /list_string_in_spec in Hdominance.
+        eauto.
+      + eapply forallb_forall in H2notin1; eauto.
+          by apply /list_string_in_spec.
+    - case_eq (p bb_id') => [ [[params insts] term] Hbb Hbbnotinterm bb_id /orP [/eqP ->| //] state /= | //].
+        by apply abstract_interpret_bb_spec_term.
+  Admitted.
 
 End AbstractInterpreter.
